Foundation/Propositional/Kripke/Logic/KP.lean
@@ -7,39 +7,41 @@ open Kripke
 open Hilbert.Kripke
 open Formula.Kripke
 
-namespace Kripke.FrameClass
+namespace Kripke
 
-protected abbrev krieselputnam : FrameClass := { F | SatisfiesKriselPutnamCondition _ F }
+protected abbrev Frame.IsKP := Frame.SatisfiesKriselPutnamCondition
 
-end Kripke.FrameClass
+protected abbrev FrameClass.KP : FrameClass := { F | F.SatisfiesKriselPutnamCondition }
+
+end Kripke
 
 
 namespace Hilbert.KP.Kripke
 
-instance sound : Sound Hilbert.KP FrameClass.krieselputnam := instSound_of_validates_axioms $ by
+instance sound : Sound Hilbert.KP FrameClass.KP := instSound_of_validates_axioms $ by
     apply FrameClass.Validates.withAxiomEFQ;
     rintro F hF _ rfl;
     replace hF := Set.mem_setOf_eq.mp hF;
-    apply validate_KrieselPutnam_of_KrieselPutnamCondition
+    apply validate_axiomKrieselPutnam_of_satisfiesKrieselPutnamCondition
 
-instance consistent : Entailment.Consistent Hilbert.KP := consistent_of_sound_frameclass FrameClass.krieselputnam $ by
+instance consistent : Entailment.Consistent Hilbert.KP := consistent_of_sound_frameclass FrameClass.KP $ by
   use whitepoint;
   apply Set.mem_setOf_eq.mpr;
   infer_instance
 
-instance canonical : Canonical Hilbert.KP FrameClass.krieselputnam := ⟨by
+instance canonical : Canonical Hilbert.KP FrameClass.KP := ⟨by
   apply Set.mem_setOf_eq.mpr;
   infer_instance;
 ⟩
 
-instance complete : Complete Hilbert.KP FrameClass.krieselputnam := inferInstance
+instance complete : Complete Hilbert.KP FrameClass.KP := inferInstance
 
 end Hilbert.KP.Kripke
 
 
 namespace Logic.KP
 
-lemma Kripke.krieselputnam : Logic.KP = Kripke.FrameClass.krieselputnam.logic := eq_Hilbert_Logic_KripkeFrameClass_Logic
+lemma Kripke.KP : Logic.KP = FrameClass.KP.logic := eq_Hilbert_Logic_KripkeFrameClass_Logic
 
 end Logic.KP
 
